StackTyping.dfy
@@ -4,21 +4,17 @@ include "Common.dfy"
 include "StackSyntax.dfy"
 include "StackSubtyping.dfy"
 
-function method Split<A>(n: nat, v: seq<A>): (seq<A>, seq<A>)
-  requires n <= |v|
-  ensures var (xs, ys) := Split(n, v); |xs| == n && |ys| == |v| - n
+function method Split<A>(n: nat, v: List<A>): (List<A>, List<A>)
+  requires n <= Length(v)
 {
-  var xs := v[.. n];
-  var ys := v[n ..];
-  (xs, ys)
+  (Take(n, v), Drop(n, v))
 }
 
-function method Uncons<A>(v: seq<A>): (A, seq<A>)
-  requires 0 < |v|
-  ensures |Uncons(v).1| == |v| - 1
+function method Uncons<A>(v: List<A>): (A, List<A>)
+  requires 0 < Length(v)
+  ensures Length(Uncons(v).1) == Length(v) - 1
 {
-  var (xs, ys) := Split(1, v);
-  (xs[0], ys)
+  (v.Head, v.Tail)
 }
 
 function method TypeValue(v: value): Type {
@@ -29,11 +25,11 @@ function method TypeValue(v: value): Type {
 }
 
 function method TypeSigma(s: sigma): Sigma {
-  MapSeq(TypeValue, s)
+  MapList(TypeValue, s)
 }
 
 predicate method ValidStack(D: Delta, phi: phi) {
-  forall frame | frame in phi :: frame.0 in D
+  forall frame | frame in Elements(phi) :: frame.0 in D
 }
 
 function method TypeFrame(D: Delta): ((nu, sigma)) -> (Phi, Sigma) {
@@ -44,47 +40,47 @@ function method TypeFrame(D: Delta): ((nu, sigma)) -> (Phi, Sigma) {
 function method TypePhi(D: Delta, phi: phi): Phi
   requires ValidStack(D, phi)
 {
-  MkPhi(MapSeq(TypeFrame(D), phi))
+  MkPhi(MapList(TypeFrame(D), phi))
 }
 
 function method TypeOperation(o: operation): (Sigma, Type) {
   match o
-    case not => ([Bool], Bool)
-    case read(t) => ([], t)
-    case printf(format) => (SeqFromList(Lefts(format)), Unit)
+    case not => (Cons(Bool, Nil), Bool)
+    case read(t) => (Nil, t)
+    case printf(format) => (Lefts(format), Unit)
     case const(v) =>
       match v {
-        case integer(_) => ([], Int)
-        case boolean(_) => ([], Bool)
-        case unit       => ([], Unit)
+        case integer(_) => (Nil, Int)
+        case boolean(_) => (Nil, Bool)
+        case unit       => (Nil, Unit)
       }
     case binary(o) =>
       match o
-        case BoolOp(_) => ([Bool, Bool], Bool)
-        case RelOp(_)  => ([Int, Int],   Bool)
-        case MathOp(_) => ([Int, Int],   Int)
+        case BoolOp(_) => (Cons(Bool, Cons(Bool, Nil)), Bool)
+        case RelOp(_)  => (Cons(Int, Cons(Int, Nil)),   Bool)
+        case MathOp(_) => (Cons(Int, Cons(Int, Nil)),   Int)
 }
 
 function method TypeCommand(c: command, S: Sigma): Maybe<Sigma> {
   match c
     case store(n) =>
-      if n < |S| && S != []
-        then Just(S[n := S[0]][1 ..])
+      if n < Length(S)
+        then Just(ReplaceNth(n, S, S.Head).Tail)
         else Nothing
     case load(n) =>
-      if n < |S|
-        then Just([S[n]] + S)
+      if n < Length(S)
+        then Just(Cons(Nth(n, S), S))
         else Nothing
     case pop(n) =>
-      if n <= |S|
-        then Just(S[n ..])
+      if n <= Length(S)
+        then Just(Drop(n, S))
         else Nothing
     case apply(n, o) =>
-      if n <= |S|
+      if n <= Length(S)
         then var (S', S'') := Split(n, S);
              var (So, t) := TypeOperation(o);
              if S' == So
-               then Just([t] + S'')
+               then Just(Cons(t, S''))
                else Nothing
         else Nothing
 }
@@ -103,41 +99,41 @@ predicate method TypeJump(D: Delta, SigmaH: Sigma, j: jump, P: Phi) {
     case goto(n) =>
       n in D && SubPhi(D[n], P)
     case halt =>
-      0 < |P.out| &&
+      P.out != Nil &&
       var ((PhiR', SigmaH'), Phi_rest) := Uncons(P.out);
       Prefix(SigmaH, SigmaH')
     case branch(n1, n2) =>
-      0 < |P.out| &&
+      P.out != Nil &&
       n1 in D && n2 in D &&
       var ((PhiR, S), Phi_rest) := Uncons(P.out);
-      S != [] &&
+      S != Nil &&
       var (t, S') := Uncons(S);
       t == Bool &&
-      var P' := MkPhi([(PhiR, S')] + Phi_rest);
+      var P' := MkPhi(Cons((PhiR, S'), Phi_rest));
       SubPhi(D[n1], P') && SubPhi(D[n2], P')
     case call(n, nJ, nR) =>
-      0 < |P.out| &&
+      P.out != Nil &&
       nJ in D && nR in D &&
       var ((PhiR, S), Phi_rest) := Uncons(P.out);
-      n < |S| &&
+      n < Length(S) &&
       var (S1, S2) := Split(n, S);
-      SubPhi(D[nJ], MkPhi([(D[nR], S1), (PhiR, S2)] + Phi_rest))
+      SubPhi(D[nJ], MkPhi(Cons((D[nR], S1), Cons((PhiR, S2), Phi_rest))))
     case ret(n) =>
-      |P.out| >= 2 &&
+      Length(P.out) >= 2 &&
       var ((PhiR, S), Phi_rest) := Uncons(P.out);
       var ((PhiR_origin, S_origin), Phi_rest_rest)  := Uncons(Phi_rest);
-      n <= |S| &&
+      n <= Length(S) &&
       var (S_check, _) := Split(n, S);
-      SubPhi(PhiR, MkPhi([(PhiR_origin, S_check + S_origin)] + Phi_rest_rest))
+      SubPhi(PhiR, MkPhi(Cons((PhiR_origin, Append(S_check, S_origin)), Phi_rest_rest)))
 }
 
 predicate method TypeBlock(D: Delta, SigmaH: Sigma, b: block, P: Phi) {
   var (cs, j) := b;
-  0 < |P.out| &&
+  P.out != Nil &&
   var ((PhiR, S), P_rest) := Uncons(P.out);
   match TypeCommands(cs, S)
     case Nothing => false
-    case Just(S_final) => TypeJump(D, SigmaH, j, MkPhi([(PhiR, S_final)] + P_rest))
+    case Just(S_final) => TypeJump(D, SigmaH, j, MkPhi(Cons((PhiR, S_final), P_rest)))
 }
 
 predicate TypeProgram(SigmaH: Sigma, D: Delta, d: delta) {
@@ -150,6 +146,13 @@ lemma TypeCommandExpansion(c: command, S1: Sigma, S1_out: Sigma, S2: Sigma)
   requires TypeCommand(c, S1) == Just(S1_out)
   ensures  exists S2_out :: TypeCommand(c, S2) == Just(S2_out)
 {
+  PrefixProperty(S1, S2);
+  match c
+    case store(n) =>
+    case load(n) =>
+    case pop(n) =>
+    case apply(n, o) =>
+      PrefixSplit(n, S1, S2);
 }
 
 lemma TypeCommandPrefixPreservation(c: command, S1: Sigma, S2: Sigma, S1': Sigma, S2': Sigma)
@@ -158,6 +161,15 @@ lemma TypeCommandPrefixPreservation(c: command, S1: Sigma, S2: Sigma, S1': Sigma
   requires TypeCommand(c, S2) == Just(S2')
   ensures  Prefix(S1', S2')
 {
+  PrefixProperty(S1, S2);
+  match c
+    case store(n) =>
+      PrefixReplace(n, S1, S2, S1.Head);
+    case load(n) =>
+    case pop(n) =>
+      PrefixSplit(n, S1, S2);
+    case apply(n, o) =>
+      PrefixSplit(n, S1, S2);
 }
 
 lemma TypeCommandsExpansion(cs: List<command>, S1: Sigma, S1_out: Sigma, S2: Sigma)
@@ -167,11 +179,14 @@ lemma TypeCommandsExpansion(cs: List<command>, S1: Sigma, S1_out: Sigma, S2: Sig
 {
   match cs
     case Nil =>
-    case Cons(c, cs) =>
+    case Cons(c, cs') =>
       var S1' := TypeCommand(c, S1).FromJust;
-      var S2' := TypeCommand(c, S2).FromJust;
+
       TypeCommandExpansion(c, S1, S1', S2);
-      TypeCommandsExpansion(cs, S1', S1_out, S2');
+      var S2' := TypeCommand(c, S2).FromJust;
+
+      TypeCommandPrefixPreservation(c, S1, S2, S1', S2');
+      TypeCommandsExpansion(cs', S1', S1_out, S2');
 }
 
 lemma TypeBlockExpansion(D: Delta, SigmaH: Sigma, b: block, P: Phi, P': Phi)
@@ -188,22 +203,22 @@ lemma TypeBlockExpansion(D: Delta, SigmaH: Sigma, b: block, P: Phi, P': Phi)
       var S_final' := TypeCommands(cs, S').FromJust;
       match j
         case goto(n) =>
-          var Phi_final  := MkPhi([(PhiR,  S_final)]  + Phi_rest);
-          var Phi_final' := MkPhi([(PhiR', S_final')] + Phi_rest');
+          var Phi_final  := MkPhi(Cons((PhiR,  S_final),  Phi_rest));
+          var Phi_final' := MkPhi(Cons((PhiR', S_final'), Phi_rest'));
           SubPhiTransitive(D[n], Phi_final, Phi_final');
         case halt =>
         case branch(n1, n2) =>
           var (_, S_final)  := Uncons(S_final);
           var (_, S_final') := Uncons(S_final');
-          var Phi_final  := MkPhi([(PhiR,  S_final)]  + Phi_rest);
-          var Phi_final' := MkPhi([(PhiR', S_final')] + Phi_rest');
+          var Phi_final  := MkPhi(Cons((PhiR,  S_final),  Phi_rest));
+          var Phi_final' := MkPhi(Cons((PhiR', S_final'), Phi_rest'));
           SubPhiTransitive(D[n1], Phi_final, Phi_final');
           SubPhiTransitive(D[n2], Phi_final, Phi_final');
         case call(n, nJ, nR) =>
           var (S1,  S2)  := Split(n, S_final);
           var (S1', S2') := Split(n, S_final');
-          var Phi_final  := [(D[nR], S1),  (PhiR,  S2)]  + Phi_rest;
-          var Phi_final' := [(D[nR], S1'), (PhiR', S2')] + Phi_rest';
+          var Phi_final  := Cons((D[nR], S1),  Cons((PhiR,  S2),  Phi_rest));
+          var Phi_final' := Cons((D[nR], S1'), Cons((PhiR', S2'), Phi_rest'));
           SubPhiReflexive(D[nR]);
           SubPhiTransitive(D[nJ], MkPhi(Phi_final), MkPhi(Phi_final'));
         case ret(n) =>
@@ -211,15 +226,15 @@ lemma TypeBlockExpansion(D: Delta, SigmaH: Sigma, b: block, P: Phi, P': Phi)
           var (S_check', _) := Split(n, S_final');
           var ((PhiR_origin,  S_origin),  Phi_rest_rest)  := Uncons(Phi_rest);
           var ((PhiR_origin', S_origin'), Phi_rest_rest') := Uncons(Phi_rest');
-          var Phi_final  :=  MkPhi([(PhiR_origin,  S_check  + S_origin)]  + Phi_rest_rest);
-          var Phi_final' :=  MkPhi([(PhiR_origin', S_check' + S_origin')] + Phi_rest_rest');
+          var Phi_final  :=  MkPhi(Cons((PhiR_origin,  Append(S_check,  S_origin)),  Phi_rest_rest));
+          var Phi_final' :=  MkPhi(Cons((PhiR_origin', Append(S_check', S_origin')), Phi_rest_rest'));
           SubPhiTransitive(PhiR, Phi_final, Phi_final');
           SubPhiAllContravariant(P, P');
           SubPhiTransitive(PhiR', PhiR, Phi_final');
 }
 
 lemma Example()
-  ensures TypeBlock(map[0 := MkPhi([])], [], (Nil, goto(0)), MkPhi([(MkPhi([]), [])]))
+  ensures TypeBlock(map[0 := MkPhi(Nil)], Nil, (Nil, goto(0)), MkPhi(Cons((MkPhi(Nil), Nil), Nil)))
 {
 }
 
